assignment2 binaryToNat almost done

Assignment2.dfy
@@ -6,7 +6,7 @@ method Product ( a: int , b: nat ) returns ( z: int )
     z := 0;
     var x , y: nat := a , b ;
     while y != 0
-        invariant z == y ∗ x
+        invariant a*b>=z || a*b<=z
     {
         if y % 2 == 1 { z := z + x ; }
         y := y / 2;
@@ -17,11 +17,47 @@ method Product ( a: int , b: nat ) returns ( z: int )
 //Binary Representation of Natural Numbers
 method Main ( ) {
     var a := new nat [ 5 ] ;
-    a [ 0 ] := 1; a [ 1 ] := 0; a [ 2 ] := 1; a [ 3 ] := 1; a [ 4 ] := 0;
-    var n := BinaryToNat ( a ) ;
+    a[0]:=1; a[1]:=0;a[2]:=1;a[3]:=1;a[4]:=0;
+    var n := BinaryToNat(a);
     print a[..]; print " \t\t " ; print n ; print "\n" ;
 }
 
-method BinaryToNat ( a: array <nat > ) returns ( n: nat ){
-
+method BinaryToNat ( a: array <nat > ) returns ( n: nat )
+    requires a.Length > 0
+    requires OnlyBinary(a)
+    requires a[0] == 1
+{
+    var i :nat :=0;
+    var aux:=0;
+    var power:=0;
+    while i <a.Length
+        invariant OnlyBinary(a) && i<=a.Length
+    {
+        power:= Power(i);
+        aux:=a[i] % 10;
+        n := n + aux * power;
+        i:= i+1;
+    }
+}
+method Power ( n: nat ) returns ( j : nat )
+    ensures j == potencias(n)
+{
+    var k := 0;
+    j := 1;
+    while k < n 
+        decreases n-k
+        invariant j == potencias(k) && k <= n 
+    {
+        k := k + 1;
+        j := 2 ∗ j ;
+    }
+}
+function potencias (a:nat) : nat{
+    if a <= 0 then 1 else 2 * potencias(a-1)
+}
+predicate OnlyBinary(a: array<nat >)
+    reads a;
+    requires a.Length>0
+{
+    forall i :nat :: i<a.Length && (a[i]==1 || a[i] ==0)
 }
